CTree- total correctness

theories/CTree/Logic/AF.v
@@ -8,13 +8,12 @@ From Coinduction Require Import
 From CTree Require Import
   Events.Core
   CTree.Core
-  CTree.SBisim
   CTree.Equ
-  CTree.Trans
   CTree.Logic.Trans
   CTree.Logic.CanStep
   Logic.Ctl
-  Logic.Kripke.
+  Logic.Kripke
+  Logic.Setoid.
 
 Set Implicit Arguments.
 Generalizable All Variables.
@@ -40,60 +39,53 @@ Section BasicLemmas.
       eapply done_not_ktrans with (t:=t); eauto.
   Qed.
 
-  (* This lemma forces us to have finite branches.
-     Alternatively, a classical φ would also allow
-     us to work without induction on branch arity. *)
-  Lemma af_brD_aux: forall n (k: fin' n -> ctree E X) w φ,
-      (forall (i: fin' n), <( {k i}, w |= AF now φ )>) -> 
-      φ w \/ (forall i, can_step (k i) w /\
-                    (forall (t': ctree E X) w', [k i, w] ↦ [t', w'] ->
-                                           <( t', w' |= AF now φ )>)).
-  Proof.
-    induction n; intros.
-    - specialize (H Fin.F1).
-      next in H; destruct H.
-      + now left.
-      + right.
-        intro i.
-        dependent destruction i; try solve [inv i].
-        next in H.
-        destruct H; intuition.
-    - (* Need to construct [k, i] *)
-      pose proof (H Fin.F1).
-      edestruct IHn with (k:=fun (i: fin (S n)) =>
-                               k (Fin.FS i)) (φ:=φ) (w:=w).
-      + intro i.
-        apply H.
-      + now left.
-      + next in H0; destruct H0.
-        * now left.
-        * right.
-          intros.
-          dependent destruction i.
-          -- now next in H0; destruct H0.
-          -- now apply H1.
-  Qed.
-  
-  Lemma af_brD: forall n (k: fin' n -> ctree E X) w φ,
-      (forall (i: fin' n), <( {k i}, w |= AF now φ )>) ->
-      <( {BrD n k}, w |= AF now φ )>.
+  Lemma af_tau: forall (t: ctree E X) w φ,
+      <( t, w |= AF now φ )> -> 
+      <( {Tau t}, w |= AF (now φ) )>.
   Proof.
     intros.
-    apply af_brD_aux in H.
-    destruct H.
-    + next; now left.
-    + next; right.
-      next; split. 
-      * apply can_step_brD.
-        exists (Fin.F1).
-        now destruct (H Fin.F1).
-      * intros.
-        apply ktrans_brD in H0 as (i & TR).
-        destruct (H i); eauto.
+    unfold entailsF in H.
+    induction H.
+    - now next; left.
+    - Opaque entailsF.
+      destruct H0, H1; clear H H1.
+      destruct H0 as (t' & w' & TR).
+      specialize (H3 _ _ TR); cbn in H3.
+      next; right.
+      split.
+      * apply can_step_tau.
+        exists t', w'; auto.
+      * intros t_ w_ TR_.
+        rewrite ktrans_tau in TR_.
+        now apply H2.
+  Qed.
+
+  Lemma afax_tau: forall (t: ctree E X) w φ,
+      <( t, w |= AF AX now φ )> -> 
+      <( {Tau t}, w |= AF AX (now φ) )>.
+  Proof.
+    intros.
+    Transparent entailsF.
+    unfold entailsF in H.
+    induction H.
+    - destruct H.
+      next; left. 
+      split.
+      + now apply can_step_tau.
+      + intros *  TR.
+        rewrite ktrans_tau in TR.
+        now apply H0 with t'.
+    - destruct H0, H1; clear H H1.
+      next; right.
+      split.
+      + now apply can_step_tau.
+      + intros * TR.
+        rewrite ktrans_tau in TR.
+        now apply H2.
   Qed.
   
-  Lemma af_brS: forall n (k: fin' n -> ctree E X) w φ,
-      <( {BrS n k}, w |= AF now φ )> <->
+  Lemma af_br: forall n (k: fin' n -> ctree E X) w φ,
+      <( {Br n k}, w |= AF now φ )> <->
         (forall (i: fin' n), <( {k i}, w |= AF now φ )>).
   Proof.
     split; intros.
@@ -102,28 +94,19 @@ Section BasicLemmas.
         now rewrite ctl_now in *.
       + destruct H.
         apply H0.
-        apply ktrans_brS.
+        apply ktrans_br.
         apply can_step_not_done in H.
         exists i; eauto.
     - destruct (not_done_dec w).
       + next; right.
         next; split; auto.
-        * now apply can_step_brS.
+        * now apply can_step_br.
         * intros t' w' TR'.
-          apply ktrans_brS in TR' as (? & -> & -> & ?).
+          apply ktrans_br in TR' as (? & -> & -> & ?).
           apply H.
       + apply done_af with (φ:=φ) (t:= k Fin.F1) in i; auto.
         next; left.
         now apply ctl_now.
-  Qed.
-
-  Lemma af_br: forall n (k: fin' n -> ctree E X) w φ b,
-    (forall (i: fin' n), <( {k i}, w |= AF now φ )>) ->
-      <( {Br b n k}, w |= AF now φ )>.
-  Proof.
-    destruct b; intros.
-    - now apply af_brS.
-    - now apply af_brD.
   Qed.
 
   Lemma af_vis: forall (e: E) (k: encode e -> ctree E X) (_: encode e) w φ,
@@ -145,173 +128,414 @@ End BasicLemmas.
 
 Section AfIndLemma.
   Context {E: Type} {HE: Encode E} {X: Type}.
-
-  (* t, w |= WF now φ *)
-  Inductive AFNowInd(φ: World E -> Prop): ctree E X -> World E -> Prop :=
-  | AFNowIndBase: forall (t: ctree E X) (w: World E),
-      φ w ->
-      AFNowInd φ t w
-  | AFNowIndDone: forall t (x: X),
+  
+  (*| [t |= AF φ] is semantic and requires double induction, on [AF] and inside it, in
+    [ktrans]. Attempt to simplify to one induction with [AFInd] |*)
+  Inductive AFInd(φ: ctree E X -> World E -> Prop): ctree E X -> World E -> Prop :=
+  | AFIndBase: forall (t: ctree E X) (w: World E),
+      φ t w ->
+      AFInd φ t w
+  | AFIndDoneBase: forall t (x: X),
       observe t = RetF x ->
-      φ (Done x) ->
-      AFNowInd φ t Pure
-  | AFNowIndFinish: forall t (e: E) (v: encode e) (x: X),
+      φ Ctree.stuck (Done x) ->
+      AFInd φ t Pure
+  | AFIndFinishBase: forall t (e: E) (v: encode e) (x: X),
       observe t = RetF x ->
-      φ (Finish e v x) ->
-      AFNowInd φ t (Obs e v)
-  | AFNowIndBr: forall t w b n (k: fin' n -> ctree E X),
-      observe t = BrF b n k ->
-      not_done w ->
-      (forall (i: fin' n), (* can_step (k i) w ->*) AFNowInd φ (k i) w) ->
-      AFNowInd φ t w
-  | AFNowIndVis: forall (t: ctree E X) w e k (_: encode e),
+      φ Ctree.stuck (Finish e v x) ->
+      AFInd φ t (Obs e v)
+  | AFIndTau: forall t u w,
+      observe t = TauF u ->
+      AFInd φ u w ->
+      AFInd φ t w
+  |AFIndVis: forall (t: ctree E X) w e k (_: encode e),
       observe t = VisF e k ->
       not_done w ->
-      (forall (v: encode e), AFNowInd φ (k v) (Obs e v)) ->
-      AFNowInd φ t w.
+      (forall (v: encode e), AFInd φ (k v) (Obs e v)) ->
+      AFInd φ t w
+  |AFIndBr: forall n (t: ctree E X) w k,
+      observe t = BrF n k ->
+      not_done w ->
+      (forall (i: fin' n), AFInd φ (k i) w) ->
+      AFInd φ t w.
 
-  Global Instance proper_equ_afind φ:
-    Proper (equ eq ==> eq ==> iff) (AFNowInd φ).
+  Global Instance proper_equ_afind φ {HP: Proper (equ eq ==> eq ==> iff) φ}:
+    Proper (equ eq ==> eq ==> iff) (AFInd φ).
   Proof.
     unfold Proper, respectful.
     intros; subst; split; intros Hind.
     - generalize dependent y.
       induction Hind; intros.
-      + apply AFNowIndBase; auto.
-      + apply AFNowIndDone with x; auto.
-        unfold equ in H1; step in H1; cbn in H1;
-          dependent destruction H1; congruence.
-      + apply AFNowIndFinish with x; auto.
-        unfold equ in H1; step in H1; cbn in H1;
-          dependent destruction H1; congruence.
-      + step in H3; cbn in H3; rewrite H in H3.
+      + apply AFIndBase; auto.
+        now rewrite <- H0.
+      + apply AFIndDoneBase with x; auto.
+        unfold equ in H1; step in H1; cbn in H1; dependent destruction H1; congruence.
+      + apply AFIndFinishBase with x; auto.
+        unfold equ in H1; step in H1; cbn in H1; dependent destruction H1; congruence.
+      + unfold equ; step in H0; cbn in H0; rewrite H in H0.
+        dependent destruction H0.
+        apply IHHind in H0.
+        apply AFIndTau with t2; congruence.
+      + unfold equ; step in H3; cbn in H3; rewrite H in H3.
         dependent destruction H3.
-        eapply AFNowIndBr with b n k2; auto.
-        intros i.
-        apply H2 with i, H3.
-      + step in H3; cbn in H3; rewrite H in H3.
-        dependent destruction H3.
-        eapply AFNowIndVis with e k2; auto.
+        eapply AFIndVis with e k2; auto.
         intros.
         apply H2, H3.
+      + unfold equ; step in H3; cbn in H3; rewrite H in H3.
+        dependent destruction H3.
+        eapply AFIndBr; eauto. 
+        intros.
+        eapply H2 with i, H3.
     - generalize dependent x.
       induction Hind; intros.
-      + apply AFNowIndBase; auto.        
-      + apply AFNowIndDone with x; auto.
-        unfold equ in H1; step in H1; cbn in H1;
-          dependent destruction H1; congruence.
-      + apply AFNowIndFinish with x; auto.
-        unfold equ in H1; step in H1; cbn in H1;
-          dependent destruction H1; congruence.
-      + step in H3; cbn in H3; rewrite H in H3.
+      + apply AFIndBase; auto.
+        now rewrite H0.
+      + apply AFIndDoneBase with x; auto.
+        unfold equ in H1; step in H1; cbn in H1; dependent destruction H1; congruence.
+      + apply AFIndFinishBase with x; auto.
+        unfold equ in H1; step in H1; cbn in H1; dependent destruction H1; congruence.
+      + unfold equ; step in H0; cbn in H0; rewrite H in H0.
+        dependent destruction H0.
+        apply IHHind in H0.
+        apply AFIndTau with t1; congruence.
+      + unfold equ; step in H3; cbn in H3; rewrite H in H3.
         dependent destruction H3.
-        eapply AFNowIndBr with b n k1; auto.
-        intros i.
-        eapply H2 with i, H3. 
-      + step in H3; cbn in H3; rewrite H in H3.
-        dependent destruction H3.
-        eapply AFNowIndVis with e k1; auto.
+        eapply AFIndVis with e k1; auto.
         intros.
         apply H2, H3.
-  Qed.
+      + unfold equ; step in H3; cbn in H3; rewrite H in H3.
+        dependent destruction H3.
+        eapply AFIndBr; eauto. 
+        intros.
+        eapply H2 with i, H3.
+  Qed.  
 
-  Lemma afind_brD_aux: forall n (k: fin' n -> ctree E X) w φ,
-      (forall i, AFNowInd φ (k i) w) ->
-      φ w \/ (forall i, can_step (k i) w /\
-                    (forall t' w', [k i, w] ↦ [t', w'] ->
-                              AFNowInd φ t' w')).
+  Lemma af_ind_stuck_done: forall (x: X) φ,
+    AFInd φ Ctree.stuck (Done x) <->
+    φ Ctree.stuck (Done x).
   Proof.
-    induction n; intros.
-    - specialize (H Fin.F1).
-      dependent induction H.
-      + (* AFIndNow *) now left.
-      + (* AFIndDone *)
-        right; intros.
-        dependent destruction i; try solve [inv i].
-        split; unfold can_step; cbn; rewrite H.
-        * exists Ctree.stuck, (Done x).
-          now econstructor.
-        * intros * TR.
-          dependent destruction TR.
-          now apply AFNowIndBase.
-      + (* AFIndFinish *)
-        right; intros.
-        dependent destruction i; try solve [inv i].
-        split; unfold can_step; cbn; rewrite H.
-        * exists Ctree.stuck, (Finish e v x).
-          now econstructor.
-        * intros * TR.
-          dependent destruction TR.
-          now apply AFNowIndBase.
-      + (* AFIndBr *) destruct b.
-        * (* BrS *) right.
-          intro i.
-          dependent destruction i; try solve [inv i].
-          unfold can_step; cbn; setoid_rewrite H.
-          split; intros.
-          -- exists (k0 Fin.F1), w; try econstructor; auto.
-          -- admit. 
-        * (* BrD *)
-          induction n.
-          -- edestruct H2.
-  Admitted.
-
-  Lemma pull1_iff: forall {A B} (P : A -> Prop) (R : A -> B -> Prop),
-      (forall a, (exists b, R a b)-> P a) <-> (forall a b, R a b -> P a).
-    split; intros; eauto.
-    destruct H0.
-    now apply H with x.
+    split; intros.
+    - dependent induction H; auto.
+    - now apply AFIndBase.
   Qed.
 
-  Lemma pull2_iff: forall {A B C} (P : A -> B -> Prop) (R : A -> B -> C -> Prop),
-      (forall a b, (exists c, R a b c)-> P a b) <-> (forall a b c, R a b c -> P a b).
-    split; intros; eauto.
-    destruct H0.
-    now apply H with x.
-  Qed.
-
-  Lemma af_afind_aux: forall (t: ctree E X) w φ,
-    (can_step t w /\
-             (forall t' w',
-                 [t, w] ↦ [t', w'] ->
-                 AFNowInd φ t' w')) ->
-    AFNowInd φ t w.
+  Lemma af_ind_stuck_finish: forall (e: E) (v: encode e) (x: X) φ,
+    AFInd φ Ctree.stuck (Finish e v x) <->
+    φ Ctree.stuck (Finish e v x).
   Proof.
-    intros.
-    destruct H as ((t' & w' & TR) & ?).
-    pose proof (H _ _ TR).
-    generalize dependent t.
-    revert w.
-    induction H0; intros.
-    + admit.
-  Admitted.
-  
-  (* This is a super useful lemma, it allows us to do
-     induction on [AFInd] instead of two inductions on
-     [cau] and [trans] *)
+    split; intros.
+    - dependent induction H; auto.
+    - now apply AFIndBase.
+  Qed.
+
+  (* This is a super useful lemma, it allows us to do induction on [AFInd]
+     instead of two inductions on [cau] and [trans] *)
   Opaque Ctree.stuck.
   Lemma af_afind : forall (t: ctree E X) (w: World E) φ,
-       <( t, w |= AF now φ )> -> AFNowInd φ t w.
-  Proof.    
-    intros; cbn in H.
-    induction H.
-    - now apply AFNowIndBase.
+       cau true (fun _ _ => True) φ t w -> AFInd φ t w.
+  Proof.
+    intros; induction H.
+    - now apply AFIndBase.
     - destruct H0, H1; clear H H1.
       destruct H0 as (t' & w' & TR).
-      apply af_afind_aux.
-      split.
-      + now (exists t', w').
-      + intros.
-        now apply H3.
+      cbn in TR.
+      dependent induction TR.
+       + eapply AFIndTau with (u:=t0); auto.
+        eapply IHTR with (t':=t'); auto.
+        -- intros t_ w_ TR_.
+           apply H2; cbn.
+           rewrite <- x0.
+           now apply ktrans_tau.
+        -- intros t_ w_ TR_.
+           apply H3; cbn.
+           rewrite <- x0.
+           now apply ktrans_tau.
+       + observe_equ x.
+         eapply AFIndBr with (n:=n) (k:=k); auto.
+         intros j.
+         apply H3; cbn.
+         rewrite <- x0.
+         apply KtransBr with j; auto.
+       + observe_equ x.
+         eapply AFIndVis with (e:=e) (k:=k); auto.
+         intros v'.
+         apply H3; cbn.
+         rewrite <- x0.
+         apply KtransObs; auto.     
+       + apply AFIndDoneBase with (x:=x0); auto.
+         assert (TR_: [t, Pure] ↦ [Ctree.stuck, Done x0]).
+         { cbn; rewrite <- x1; apply KtransDone; auto. }
+         specialize (H3 _ _ TR_).
+         now apply af_ind_stuck_done.
+       + apply AFIndFinishBase with (x:=x0); auto.
+         assert (TR_: [t, Obs e v] ↦ [Ctree.stuck, Finish e v x0]).
+         { cbn; rewrite <- x1; apply KtransFinish; auto. }
+         specialize (H3 _ _ TR_).
+         now apply af_ind_stuck_finish.
   Qed.
-  
+
+  (* -> *)
+  Lemma afind_af {Hpr: @Productive E HE} φ
+    {HP: Proper (equ eq ==> eq ==> iff) φ}
+    {TauInv: forall (t: ctree E X) w, φ t w  -> φ (Tau t) w}
+    : forall (t: ctree E X) (w: World E),
+      AFInd φ t w -> cau true (fun _ _ => True) φ t w.
+  Proof.
+    intros; induction H.
+    - now apply MatchA.
+    - apply StepA; auto; split.
+      + exists Ctree.stuck, (Done x).
+        Opaque Ctree.stuck.
+        cbn. rewrite H.
+        apply KtransDone; auto.
+      + intros t' w' TR.
+        cbn in TR.        
+        dependent induction TR.
+        * rewrite H in x1; inv x1.
+        * rewrite H in x1; inv x1.
+        * rewrite H in x1; inv x1.
+        * observe_equ x.
+          rewrite <- Eqt, H1.
+          rewrite <- x2 in H.
+          inv H.
+          now apply MatchA.
+    - apply StepA; auto; split.
+      + exists Ctree.stuck, (Finish e v x).
+        Opaque Ctree.stuck.
+        cbn. rewrite H.
+        apply KtransFinish; auto.
+      + intros t' w' TR.
+        cbn in TR.
+        dependent induction TR.
+        * rewrite H in x1; inv x1.
+        * rewrite H in x1; inv x1.
+        * rewrite H in x1; inv x1.
+        * observe_equ x.
+          rewrite <- Eqt, H1.
+          rewrite <- x2 in H.
+          inv H.
+          now apply MatchA.
+    - observe_equ H.
+      rewrite Eqt; clear Eqt.
+      destruct IHAFInd.
+      + apply MatchA.
+        (* TauInv here *)
+        now apply TauInv.
+      + destruct H2.
+        apply StepA; auto.
+        split.
+        * now apply can_step_tau.
+        * intros t' w' TR.
+          apply H3.
+          now rewrite ktrans_tau in TR.
+    - observe_equ H.
+      rewrite Eqt; clear Eqt.
+      apply StepA; auto; split.
+      + now apply can_step_vis.
+      + intros t' w' TR.
+        apply ktrans_vis in TR as (v & -> & <- & ?).
+        eapply H2.
+    - observe_equ H.
+      rewrite Eqt; clear Eqt.
+      apply StepA; auto; split.
+      + now apply can_step_br.
+      + intros t' w' TR.
+        apply ktrans_br in TR as (v & -> & <- & ?).
+        eapply H2.
+  Qed.
 End AfIndLemma.
+
+Section AfDoneIndLemma.
+  Context {E: Type} {HE: Encode E} {X: Type}
+    (φ: X -> World E -> Prop).
+
+  (* t |= AF AX done R *)
+  Inductive AFDoneInd: ctree E X -> World E -> Prop :=
+  | AFDoneDoneBase: forall t (x: X),
+      observe t = RetF x ->
+      φ x Pure ->
+      AFDoneInd t Pure
+  | AFDoneFinishBase: forall t (e: E) (v: encode e) (x: X),
+      observe t = RetF x ->
+      φ x (Obs e v) ->
+      AFDoneInd t (Obs e v)
+  | AFDoneIndTau: forall t u w,
+      observe t = TauF u ->
+      AFDoneInd u w ->
+      AFDoneInd t w
+  |AFDoneIndVis: forall (t: ctree E X) w e k (_: encode e),
+      observe t = VisF e k ->
+      not_done w ->
+      (forall (v: encode e), AFDoneInd (k v) (Obs e v)) ->
+      AFDoneInd t w
+  |AFDoneIndBr: forall (t: ctree E X) w n (k: fin' n -> _),
+      observe t = BrF n k ->
+      not_done w ->
+      (forall (i: fin' n), AFDoneInd (k i) w) ->
+      AFDoneInd t w.
+
+  Global Instance proper_equ_afdoneind:
+    Proper (equ eq ==> eq ==> iff) AFDoneInd.
+  Proof.
+    unfold Proper, respectful.
+    intros; subst; split; intros Hind.
+    - generalize dependent y.
+      induction Hind; intros.
+      + apply AFDoneDoneBase with x; auto.
+        rewrite <- H.
+        unfold equ in H.
+        step in H1; cbn in H1; dependent destruction H1;
+          congruence.
+      + apply AFDoneFinishBase with x; auto.
+        rewrite <- H.
+        step in H1; cbn in H1; dependent destruction H1;
+          congruence.
+      + unfold equ; step in H0; cbn in H0; rewrite H in H0.
+        dependent destruction H0.
+        apply IHHind in H0.
+        apply AFDoneIndTau with t2; congruence.
+      + unfold equ; step in H3; cbn in H3; rewrite H in H3.
+        dependent destruction H3.
+        eapply AFDoneIndVis with e k2; auto; intros.
+        apply H2, H3.
+      + unfold equ; step in H3; cbn in H3; rewrite H in H3.
+        dependent destruction H3.
+        eapply AFDoneIndBr with _ k2; auto; intros.
+        apply H2 with i, H3.
+    - generalize dependent x.
+      induction Hind; intros.
+      + apply AFDoneDoneBase with x; auto.
+        rewrite <- H.
+        unfold equ in H.
+        step in H1; cbn in H1; dependent destruction H1;
+          congruence.
+      + apply AFDoneFinishBase with x; auto.
+        rewrite <- H.
+        step in H1; cbn in H1; dependent destruction H1;
+          congruence.
+      + unfold equ; step in H0; cbn in H0; rewrite H in H0.
+        dependent destruction H0.
+        apply IHHind in H0.
+        apply AFDoneIndTau with t1; congruence.
+      + unfold equ; step in H3; cbn in H3; rewrite H in H3.
+        dependent destruction H3.
+        eapply AFDoneIndVis with e k1; auto; intros.
+        apply H2, H3.
+      + unfold equ; step in H3; cbn in H3; rewrite H in H3.
+        dependent destruction H3.
+        eapply AFDoneIndBr with _ k1; auto; intros.
+        apply H2 with i, H3.
+  Qed.
+
+  Lemma afdoneind_stuck: forall w,
+      ~ (AFDoneInd Ctree.stuck w).
+  Proof.
+    intros * Hcontra.
+    dependent induction Hcontra; eauto.
+  Qed.
+
+  Lemma afdone_ind: forall (t: ctree E X) w,
+      <( t, w |= AF AX done φ )> ->
+      AFDoneInd t w.
+  Proof.
+    intros; induction H.
+    - next in H.
+      destruct H as [(t' & w' & TR) H].
+      cbn in TR.
+      dependent induction TR.
+      + eapply AFDoneIndTau with (u:=t0); auto.
+        eapply IHTR; auto.
+        intros t_ w_ TR_.
+        apply H; cbn.
+        rewrite <- x0.
+        now apply ktrans_tau.
+      + eapply AFDoneIndBr; eauto.
+        intros v'.
+        assert (TR: ktrans_ (observe t) w (observe (k v')) w).
+        { rewrite <- x0; apply ktrans_br; exists v'; eauto. }
+        specialize (H1 _ _ TR).
+        rewrite ctl_done in H1.
+        inv H1; inv H.
+      + eapply AFDoneIndVis; eauto.
+        intros v'.
+        assert (TR: ktrans_ (observe t) w (observe (k v')) (Obs e v')).
+        { rewrite <- x0; apply ktrans_vis; exists v'; eauto. }
+        specialize (H1 _ _ TR).
+        rewrite ctl_done in H1.
+        inv H1.
+      + eapply AFDoneDoneBase with (x:=x0); auto.
+        assert (TR: ktrans_ (observe t) Pure (observe Ctree.stuck) (Done x0)).
+        { rewrite <- x1; econstructor; auto. }
+        specialize (H0 _ _ TR).
+        rewrite ctl_done in H0.
+        now dependent destruction H0.
+      + eapply AFDoneFinishBase with (x:=x0); auto.
+        assert (TR: ktrans_ (observe t) (Obs e v) (observe Ctree.stuck) (Finish e v x0)).
+        { rewrite <- x1; econstructor; auto. }
+        specialize (H0 _ _ TR).
+        rewrite ctl_done in H0.
+        now dependent destruction H0.
+    -  destruct H0, H1; clear H H1.
+       destruct H0 as (t' & w' & TR).
+       cbn in TR.
+       dependent induction TR.
+       + eapply AFDoneIndTau with (u:=t0); auto.
+        eapply (IHTR) with (t':=t'); auto.
+        -- intros t_ w_ TR_.
+           apply H2; cbn.
+           rewrite <- x0.
+           now apply ktrans_tau.
+        -- intros t_ w_ TR_.
+           apply H3; cbn.
+           rewrite <- x0.
+           now apply ktrans_tau.
+       + observe_equ x.
+         eapply AFDoneIndBr with n k; auto.
+         intros i'.
+         apply H3; cbn.
+         rewrite <- x0.
+         apply KtransBr with i'; auto.
+       + observe_equ x.
+         eapply AFDoneIndVis with (e:=e) (k:=k); auto.
+         intros v'.
+         apply H3; cbn.
+         rewrite <- x0.
+         apply KtransObs; auto.
+      + apply AFDoneDoneBase with (x:=x0); auto.
+        assert (TR_: ktrans_ (observe t) Pure (observe Ctree.stuck) (Done x0)).
+        { rewrite <- x1; apply KtransDone; auto. }
+        specialize (H3 _ _ TR_).
+        now apply afdoneind_stuck in H3.
+      + apply AFDoneFinishBase with (x:=x0); auto.
+        assert (TR_: ktrans_ (observe t) (Obs e v) (observe Ctree.stuck) (Finish e v x0)).
+        { rewrite <- x1; apply KtransFinish; auto. }
+        specialize (H3 _ _ TR_).
+        now apply afdoneind_stuck in H3.
+  Qed.
+
+  Lemma af_ret_inv: forall (x: X) w R,
+      <( {Ret x}, w |= AF (AX done R) )> ->
+      R x w.
+  Proof.
+    intros.
+    apply af_afind in H.
+    dependent induction H.
+    - destruct H.
+      destruct H as (t' & w' & TR).
+      specialize (H0 _ _ TR).
+      inv H0; destruct w; cbn in TR; dependent destruction TR; auto.
+    - destruct H0.
+      apply can_step_not_done in H.
+      inv H.
+    - destruct H0.
+      apply can_step_not_done in H.
+      inv H.
+  Qed.
+
+End AfDoneIndLemma.
 
 Section CtlAfBind.
   Context {E: Type} {HE: Encode E}.
 
-  (* LEF: This lemma is not provable with [can_step]
-     in AFNowBr *)
   Lemma af_stuck{X}: forall φ w,
       φ w <->
       <( {Ctree.stuck: ctree E X}, w |= AF now φ )>.
@@ -322,9 +546,7 @@ Section CtlAfBind.
       apply af_afind in H.
       Transparent Ctree.stuck.
       induction H; subst; auto; cbn in *;
-        dependent destruction H. 
-      apply H2; auto.
-      exact Fin.F1.
+        dependent destruction H; auto.      
   Qed.
 
   Typeclasses Transparent equ.
@@ -346,12 +568,16 @@ Section CtlAfBind.
       inv H0.
     - (* Tau *)
       observe_equ H.
-      rewrite Eqt, bind_br.
-      apply af_br; eauto.
+      rewrite Eqt, bind_tau.
+      apply af_tau; eauto.
     - (* Vis *)
       observe_equ H.
       rewrite Eqt, bind_vis.
       apply af_vis; eauto.
+    - (* Br *)
+      observe_equ H.
+      rewrite Eqt, bind_br.
+      apply af_br; eauto.      
   Qed.
 
   Theorem af_bind_pure{X Y}: forall (t: ctree E Y) (k: Y -> ctree E X) w,
@@ -370,12 +596,16 @@ Section CtlAfBind.
       inv H0.
     - (* Tau *)
       observe_equ H.
-      rewrite Eqt, bind_br.
-      apply af_br; eauto.
+      rewrite Eqt, bind_tau.
+      apply af_tau; eauto.
     - (* Vis *)
       observe_equ H.
       rewrite Eqt, bind_vis.
       apply af_vis; eauto.
+    - (* Br *)
+      observe_equ H.
+      rewrite Eqt, bind_br.
+      apply af_br; eauto.   
   Qed.
   
   Lemma can_step_bind_r{X Y}: forall (t: ctree E Y) (k: Y -> ctree E X) w R,      
@@ -384,7 +614,7 @@ Section CtlAfBind.
       can_step (x <- t ;; k x) w.
   Proof.    
     intros.
-    apply af_afind in H.
+    apply afdone_ind in H.
     generalize dependent k.
     induction H; intros; observe_equ H; rewrite Eqt.
     - (* Done x *)
@@ -399,11 +629,14 @@ Section CtlAfBind.
     - (* Vis *)
       rewrite bind_vis.
       apply can_step_vis; auto.
+    - (* Br *)
+      rewrite bind_br.
+      apply can_step_br; auto.
   Qed.
   Hint Resolve can_step_bind_r: ctl.
 
-  Theorem af_bind_r{X Y}: forall (t: itree E Y)
-                            (k: Y -> itree E X) w φ R,
+  Theorem af_bind_r{X Y}: forall (t: ctree E Y)
+                            (k: Y -> ctree E X) w φ R,
       <( t, w |= AF AX done R )> ->
       (forall (y: Y) w, R y w -> not_done w ->
                    <( {k y}, w |= AF now φ )>) ->
@@ -425,6 +658,9 @@ Section CtlAfBind.
     - (* Vis *)
       rewrite bind_vis.
       apply af_vis; eauto with ctl.
+    - (* Br *)
+      rewrite bind_br.
+      apply af_br; eauto with ctl.
   Qed.
 
 End CtlAfBind.
@@ -436,7 +672,7 @@ Section CtlAfIter.
   (* [Ri: I -> World E -> Prop] loop invariant (left).
      [Rr: X -> World E -> Prop] loop postcondition (right).
      [Rv: (I * World E) -> (I * World E) -> Prop)] loop variant (left). *)
-  Lemma af_iter{X I} Ri Rr (Rv: relation (I * World E)) (i: I) w (k: I -> itree E (I + X)):
+  Lemma af_iter{X I} Ri Rr (Rv: relation (I * World E)) (i: I) w (k: I -> ctree E (I + X)):
       (forall (i: I) w, Ri i w ->
                    <( {k i}, w |= AF AX done {fun (x: I + X) w' =>
                                              match x with
@@ -445,7 +681,7 @@ Section CtlAfIter.
                                              end})>) ->
       well_founded Rv ->
       Ri i w ->
-      <( {Itree.iter k i}, w |= AF done Rr )>.
+      <( {Ctree.iter k i}, w |= AF done Rr )>.
   Proof.      
     intros H WfR Hi.
     generalize dependent k.
@@ -477,7 +713,7 @@ Section CtlAfIter.
       + now apply can_step_ret.
       + intros t_ w_ TR_.
         inv Hd.
-        * apply ktrans_pure in TR_ as (-> & ->).
+        * cbn in TR_. dependent destruction TR_. 
           next; left.
           rewrite ctl_done.
           now constructor.
@@ -487,3 +723,5 @@ Section CtlAfIter.
           now constructor.          
   Qed.
 End CtlAfIter.
+
+
