theories/CTree/Interp/State.v
@@ -55,8 +55,9 @@ Notation interp_state_ h t s :=
   (match observe t with
    | RetF r => Ret (r, s)
    | VisF e k => (runStateT (h.(handler) e) s) >>=
-                  (fun '(x, s') => guard (interp_state h (k x) s'))
-   | BrF b n k => Br b n (fun xs => guard (interp_state h (k xs) s))
+                  (fun '(x, s') => Tau (interp_state h (k x) s'))
+   | TauF t => Tau (interp_state h t s)
+   | BrF n k => Br n (fun xs => Tau (interp_state h (k xs) s))
    end)%function.
 
 Lemma unfold_interp_state `{Encode F} `(h: E ~> stateT W (ctree F))
@@ -74,6 +75,8 @@ Proof.
     rewrite ?bind_bind, ?bind_branch.
     apply br_equ; intros.
     now cbn; rewrite ?bind_ret_l.
+  - rewrite ?bind_bind, ?bind_ret_l; cbn.
+    reflexivity.
   - rewrite ?bind_bind.
     upto_bind_equ.
     destruct x1 eqn:Hx1.
@@ -95,9 +98,12 @@ Proof.
     apply H2.
   - cbn.
     constructor; intros.
+    apply IH; auto.
+  - cbn.
+    constructor.
+    intros i.
     step.
-    econstructor; intros FF.
-    dependent destruction FF; try inversion FF.
+    econstructor.
     apply IH; auto.
     apply H2.
 Qed.
@@ -111,26 +117,34 @@ Qed.
 Lemma interp_state_vis `{Encode F} `(h: E ~> stateT W (ctree F)) {X}  
   (e : E) (k : encode e -> ctree E X) (w : W) :
   interp_state h (Vis e k) w ≅ runStateT (h.(handler) e) w >>=
-    (fun '(x, w') => guard (interp_state h (k x) w')).
+    (fun '(x, w') => Tau (interp_state h (k x) w')).
 Proof.
   rewrite unfold_interp_state; reflexivity.
 Qed.
 
 Lemma interp_state_trigger `{Encode F} `(h: E ~> stateT W (ctree F))
   (e : E) (w : W) :
-  interp_state h (Ctree.trigger e) w ≅ runStateT (h.(handler) (resum e)) w >>= fun x => guard (Ret x).
+  interp_state h (Ctree.trigger e) w ≅ runStateT (h.(handler) (resum e)) w >>= fun x => Tau (Ret x).
 Proof.
   unfold Ctree.trigger.
   rewrite interp_state_vis.
   upto_bind_equ.
   destruct x1.
-  setoid_rewrite interp_state_ret.
+  step; constructor.
+  rewrite interp_state_ret.
   reflexivity.
 Qed.  
 
 Lemma interp_state_br `{Encode F} `(h: E ~> stateT W (ctree F)) {X}
-  (n : nat) (k : fin' n -> ctree E X) (w : W) b :
-  interp_state h (Br b n k) w ≅ Br b n (fun x => guard (interp_state h (k x) w)).
+  (n : nat) (k : fin' n -> ctree E X) (w : W) :
+  interp_state h (Br n k) w ≅ Br n (fun x => Tau (interp_state h (k x) w)).
+Proof.
+  rewrite !unfold_interp_state; reflexivity.
+Qed.
+
+Lemma interp_state_tau `{Encode F} `(h: E ~> stateT W (ctree F)) {X}
+  (t : ctree E X) (w : W) :
+  interp_state h (Tau t) w ≅ Tau ((interp_state h t w)).
 Proof.
   rewrite !unfold_interp_state; reflexivity.
 Qed.
@@ -145,6 +159,7 @@ Proof.
   destruct (observe t) eqn:?.
   - rewrite interp_state_ret in H0. step in H0. inv H0. split; reflexivity.
   - rewrite interp_state_br in H0. step in H0. inv H0.
+  - rewrite interp_state_tau in H0. step in H0. inv H0.
   - rewrite interp_state_vis in H0. apply ret_equ_bind in H0 as (? & ? & ?).
     destruct x.
     step in H1.
@@ -172,17 +187,22 @@ Proof.
     constructor; intro i.
     step; econstructor; intros.
     apply IH.
+  - rewrite interp_state_tau.
+    rewrite bind_tau.
+    constructor.
+    apply IH.
   - rewrite interp_state_vis, bind_bind.
     upto_bind_equ; destruct x.
-    rewrite bind_guard.
-    constructor; intros ?; apply IH.
+    rewrite bind_tau.
+    constructor.
+    apply IH.
 Qed.
 
 Lemma interp_state_unfold_iter `{Encode F} `(h : E ~> stateT W (ctree F)) {I R}
   (k : I -> ctree E (I + R)) (i: I) (s: W) :
   interp_state h (iter k i) s ≅ interp_state h (k i) s >>= fun '(x, s) =>
       match x with
-      | inl l => guard (guard (interp_state h (iter k l) s))
+      | inl l => Tau (interp_state h (iter k l) s)
       | inr r => Ret (r, s)
       end.
 Proof.
@@ -190,8 +210,9 @@ Proof.
   setoid_rewrite unfold_iter.
   rewrite interp_state_bind.
   upto_bind_equ.
+  unfold iter, MonadIter_ctree. 
   destruct x1 as [[l | r] s'].
-  - rewrite interp_state_br.
+  - rewrite interp_state_tau.
     reflexivity.
   - rewrite interp_state_ret.
     reflexivity.
