theories/CTree/Rutt/Core.v
@@ -1,0 +1,542 @@
+From Coq Require Import
+     Basics
+     Program.Equality
+     Eqdep
+     Classes.SetoidClass
+     Classes.RelationPairs.
+
+From Coinduction Require Import
+     coinduction rel tactics.
+
+From CTree Require Import
+  CTree.Core.
+
+(*| Equivalence up to tau on ctrees |*)
+Section Rutt.
+  Context {E: Type} {HE: Encode E}
+    {X1 X2 : Type} (RE: forall (e1 e2: E), encode e1 -> encode e2 -> Prop)
+    (RR : X1 -> X2 -> Prop).
+
+  Inductive ruttF (eq : ctree E X1 -> ctree E X2 -> Prop) :
+    ctree' E X1 -> ctree' E X2 -> Prop :=
+    | RuttRet x y:
+      RR x y ->
+      ruttF eq (RetF x) (RetF y)
+    | RuttVis (e1 e2: E) (k1: encode e1 -> _) (k2: encode e2 -> _):
+      (forall x y, RE e1 e2 x y -> eq (k1 x) (k2 y)) ->
+      ruttF eq (VisF e1 k1) (VisF e2 k2)
+    | RuttTau t1 t2:
+      eq t1 t2 ->
+      ruttF eq (TauF t1) (TauF t2)
+    | RuttTauL t1 t2:
+      ruttF eq (observe t1) t2 ->
+      ruttF eq (TauF t1) t2
+    | RuttTauR t1 t2:
+      ruttF eq t1 (observe t2) ->
+      ruttF eq t1 (TauF t2)            
+    | RuttBr {n} k1 k2:
+      (forall (x: fin' n), eq (k1 x) (k2 x)) ->
+      ruttF eq (BrF n k1) (BrF n k2).
+  Hint Constructors ruttF: core.
+
+  Program Definition frutt: mon (ctree E X1 -> ctree E X2 -> Prop) :=
+    {|body eq t1 t2 :=  ruttF eq (observe t1) (observe t2) |}.
+  Next Obligation.
+    unfold pointwise_relation, Basics.impl,
+      Proper, respectful.
+    cbn; intros; dependent induction H0;
+      rewrite <- ?x2, <- ?x1, <- ?x; eauto.
+  Qed.
+End Rutt.
+
+Definition rutt {E} {HE:Encode E} {X1 X2} RR RE :=
+  (gfp (@frutt E HE X1 X2 RR RE)).
+
+#[global] Hint Constructors ruttF: core.
+
+Ltac fold_rutt_in H:=
+  multimatch type of H with
+  | context[gfp (@frutt ?E ?HE ?X1 ?X2 ?RR ?RE)] =>
+      fold (@rutt E HE X1 X2 RR RE) in H
+  end.
+
+Ltac fold_rutt :=
+  match goal with
+  | |- context[gfp (@frutt ?E ?HE ?X1 ?X2 ?RR ?RE)] =>
+      fold (@rutt E HE X1 X2 RR RE)
+  end.
+
+Ltac __coinduction_rutt R H :=
+  unfold rutt; apply_coinduction; intros R H.
+
+Ltac __step_rutt := unfold rutt; step; fold_rutt.
+
+#[global] Tactic Notation "step" := __step_rutt || step.
+#[global] Tactic Notation "coinduction" simple_intropattern(R) simple_intropattern(H) := __coinduction_rutt R H.
+
+Ltac __step_rutt_in H := unfold rutt in H; step in H; fold_rutt_in H.
+
+#[global] Tactic Notation "step" "in" ident(H) :=
+  __step_rutt_in H || step in H.
+
+Definition eq_enc{E} {HE: Encode E} (e1 e2: E) (x: encode e1) (y: encode e2): Prop := eq_dep E encode e1 x e2 y.
+Arguments eq_enc /.
+
+Check rutt.
+Infix "~" := (rutt eq_enc eq) (at level 70): ctree_scope.
+
+(** The associated companions *)
+Notation rt RE RR  := (t (frutt RE RR)).
+Notation rT RE RR := (T (frutt RE RR)).
+Notation rbt RE RR := (bt (frutt RE RR)).
+Notation rbT RE RR := (bT (frutt RE RR)).
+
+Notation "t [≅] u" := (rt eq_enc eq _ t u) (at level 79): ctree_scope.
+Notation "t {≅} u" := (rbt eq_enc eq _ t u) (at level 79): ctree_scope.
+Notation "t {{≅}} u" := (ruttF eq_enc eq (rutt eq_enc) t u)
+                          (at level 79): ctree_scope.
+
+Section RuttHomogenousTheory.
+  Context {E: Type} {HE: Encode E} {X : Type}
+    (RE: forall (e1 e2: E), encode e1 -> encode e2 -> Prop) (RR: X -> X -> Prop).
+  Notation rT  := (T (frutt (E := E) (HE:=HE) (X1:=X) (X2:=X) RE RR)).
+  Notation rt  := (t (frutt (E := E) (HE:=HE) (X1:=X) (X2:=X) RE RR)).
+  Notation rbt := (bt (frutt (E := E) (HE:=HE) (X1:=X) (X2:=X) RE RR)).
+
+  (** [const eq] is compatible: up-to reflexivity is valid *)
+  Lemma refl_t {HR: Reflexive RR}: const eq <= rt.
+  Proof.
+    apply leq_t.  intro.
+    cbn.
+    intros p ? <-.
+    desobs p; auto.
+    econstructor; intros.
+    
+  Admitted.
+
+  (** [converse] is compatible: up-to symmetry is valid *)
+  Lemma converse_t {HR: Symmetric RR}: converse <= et.
+  Proof.
+    apply leq_t; intros S x y H; cbn. destruct H; auto.
+  Qed.
+
+  (** [squaring] is compatible: up-to transitivity is valid *)
+  Lemma square_t {HR: Reflexive RR} {HT: Transitive RR}: square <= et.
+  Proof.
+    apply leq_t.
+    intros S x z [y xy yz]; cbn.
+    inversion xy; inversion yz; try (exfalso; congruence).
+    - constructor.
+      rewrite <-H0 in H2.
+      rewrite H1, <-H4.
+      now inversion H2.
+    - rewrite <- H0 in H2.
+      dependent destruction H2.
+      eauto.
+    - rewrite <- H0 in H2.
+      dependent destruction H2.
+      eauto.
+    - rewrite <- H0 in H2.
+      dependent destruction H2.
+      eauto.
+  Qed.
+
+  #[global] Instance Equivalence_et {HR: Equivalence RR} S: Equivalence (et S).
+  Proof. apply Equivalence_t. apply refl_t. apply square_t. apply converse_t. Qed.
+  #[global] Instance Equivalence_eT  {HR: Equivalence RR} f S: Equivalence (eT f S).
+  Proof. apply Equivalence_T. apply refl_t. apply square_t. apply converse_t. Qed.
+  #[global] Instance Equivalence_ebt  {HR: Equivalence RR} S: Equivalence (ebt S).
+  Proof. apply Equivalence_bt. apply refl_t. apply square_t. apply converse_t. Qed.
+  #[global] Instance Equivalence_equ  {HR: Equivalence RR}: Equivalence (@equ E HE X X RR) | 1.
+  Proof. apply Equivalence_et. Qed.
+
+  #[global] Instance Reflexive_equb (equ : ctree E X -> ctree E X -> Prop) :
+    Reflexive RR -> Reflexive equ -> Reflexive (equF RR equ).
+  Proof.
+    red. destruct x; auto.
+  Qed.
+
+End EquTheory.
+Local Open Scope ctree_scope.
+#[global] Hint Constructors equF: core.
+
+#[global] Instance equ_eq_equ_impl {E R} {HE: Encode E}:
+  Proper (equ eq ==> equ eq ==> flip impl) (@equ E _ R R eq).
+Proof.
+  unfold Proper, respectful, flip, impl; cbn.
+  unfold equ; coinduction RR IH.  
+  intros t t' EQt u u' EQu EQ.
+  step in EQt.
+  step in EQu.
+  step in EQ.
+  cbn*; cbn in *; inv EQt; rewrite <-H0 in EQ.
+  - inv EQ.
+    rewrite <-H2 in EQu.
+    inv EQu; auto.
+  - dependent destruction EQ.
+    rewrite <- x in EQu.
+    dependent destruction EQu.
+    rewrite <- x.
+    constructor.
+    intro x1; rewrite H1, H0, <- H.
+    reflexivity.
+  - dependent destruction EQ.
+    rewrite <- x in EQu.
+    dependent destruction EQu.
+    rewrite <- x.
+    constructor.
+    eapply IH; eauto.
+  - dependent destruction EQ.
+    cbn.
+    rewrite <- x in EQu.
+    dependent destruction EQu.
+    rewrite <- x.
+    constructor.
+    intro x1; rewrite H1, H0, <- H.
+    reflexivity.
+Qed.
+
+#[global] Instance equ_eq_equ_goal {E R} {HE: Encode E}:
+  Proper (equ eq ==> equ eq ==> impl) (@equ E _ R R eq).
+Proof.
+  unfold Proper, respectful, flip, impl; cbn.
+  unfold equ; coinduction RR IH.  
+  intros t t' EQt u u' EQu EQ.
+  step in EQt.
+  step in EQu.
+  step in EQ.
+  cbn*; cbn in *; inv EQt; rewrite <- H in EQ.
+  - inv EQ; auto.
+    rewrite <- H2 in EQu.
+    inv EQu; auto.
+  - dependent destruction EQ.
+    rewrite <- x in EQu.
+    dependent destruction EQu.
+    rewrite <- x.
+    constructor.
+    intro x1. rewrite <- H, <- H1, H0.
+    reflexivity.
+  - dependent destruction EQ.
+    cbn.
+    rewrite <- x in EQu.
+    dependent destruction EQu.
+    rewrite <- x.
+    constructor; eauto.
+  - dependent destruction EQ.
+    cbn.
+    rewrite <- x in EQu.
+    dependent destruction EQu.
+    rewrite <- x.
+    constructor.
+    intro x1; rewrite <- H, <- H1, <- H0.
+    reflexivity.
+Qed.
+
+(** Shallow [observing]: Lift relations through [observe]. *)
+Record observing {E R} {HE: Encode E}
+           (eq_ : ctree' E R -> ctree' E R -> Prop)
+           (t1 : ctree E R) (t2 : ctree E R) : Prop :=
+  observing_intros
+  { observing_observe : eq_ (observe t1) (observe t2) }.
+#[global] Hint Constructors observing: core.
+Arguments observing_observe {E R HE eq_ t1 t2}.
+
+Section observing_relations.
+  Context {E : Type} {HE: Encode E} {R : Type}.
+  Variable (eq_ : ctree' E R -> ctree' E R -> Prop).
+
+  #[global] Instance observing_observe_ :
+    Proper (observing eq_ ==> eq_) observe.
+  Proof. intros ? ? []; cbv; auto. Qed.
+
+  #[global] Instance observing_go : Proper (eq_ ==> observing eq_) go.
+  Proof. cbv; auto. Qed.
+
+  #[global] Instance monotonic_observing eq_' :
+    subrelation eq_ eq_' ->
+    subrelation (observing eq_) (observing eq_').
+  Proof. intros ? ? ? []; cbv; eauto. Qed.
+
+  #[global] Instance Equivalence_observing :
+    Equivalence eq_ -> Equivalence (observing eq_).
+  Proof.
+    intros []; split; cbv; auto.
+    - intros ? ? []; auto.
+    - intros ? ? ? [] []; eauto.
+  Qed.
+
+End observing_relations.
+
+(** ** Unfolding lemmas for [bind] *)
+#[global] Instance observing_bind {E R S} {HE: Encode E}:
+  Proper (observing eq ==> eq ==> observing eq) (@Ctree.bind E HE R S).
+Proof.
+  repeat intro; subst. constructor.
+  unfold observe. cbn.
+  rewrite (observing_observe H). reflexivity.
+Qed.
+
+Lemma bind_ret_ {E R S} {HE: Encode E} (r : R) (k : R -> ctree E S) :
+  observing eq (Ctree.bind (Ret r) k) (k r).
+Proof. constructor; reflexivity. Qed.
+
+Lemma bind_guard_ {E R} {HE: Encode E} U t (k: U -> ctree E R) :
+  observing eq (Ctree.bind (Tau t) k) (Tau (Ctree.bind t k)).
+Proof. constructor; reflexivity. Qed.
+
+Lemma bind_br_ {E R} {HE: Encode E} n U (bk: fin' n -> ctree E U) (k: U -> ctree E R) :
+  observing eq (Ctree.bind (Br n bk) k) (Br n (fun i => Ctree.bind (bk i) k)).
+Proof. constructor; reflexivity. Qed.
+
+Lemma bind_vis_ {E R U} {HE: Encode E} (e: E) (ek: encode e -> ctree E U) (k: U -> ctree E R) :
+  observing eq
+    (Ctree.bind (Vis e ek) k)
+    (Vis e (fun x => Ctree.bind (ek x) k)).
+Proof. constructor; reflexivity. Qed.
+
+(** Unfolding lemma for [iter]. There is also a variant [unfold_iter]
+    without [Tau]. *)
+Lemma unfold_aloop_ {E X Y} {HE: Encode E} (f : X -> ctree E (X + Y)) (x : X) :
+  observing eq
+    (Ctree.iter f x)
+    (Ctree.bind (f x) (fun lr => on_left lr l (Tau (Ctree.iter f l)))).
+Proof. constructor; reflexivity. Qed.
+
+(** ** [going]: Lift relations through [go]. *)
+
+(** Shallow [going] *)
+Inductive going {E R1 R2} {HE: Encode E} (r : ctree E R1 -> ctree E R2 -> Prop)
+          (ot1 : ctree' E R1) (ot2 : ctree' E R2) : Prop :=
+| going_intros : r (go ot1) (go ot2) -> going r ot1 ot2.
+#[global] Hint Constructors going: core.
+
+Lemma observing_going {E R} {HE: Encode E} (eq_ : ctree' E R -> ctree' E R -> Prop) ot1 ot2 :
+  going (observing eq_) ot1 ot2 <-> eq_ ot1 ot2.
+Proof.
+  split; auto; intros [[]]; auto.
+Qed.
+
+Section going_relations.
+
+  Context {E : Type} {HE: Encode E} {R : Type}.
+  Variable (eq_ : ctree E R -> ctree E R -> Prop).
+
+  #[global] Instance going_go : Proper (going eq_ ==> eq_) go.
+  Proof. intros ? ? []; auto. Qed.
+
+#[global] Instance monotonic_going eq_' :
+  subrelation eq_ eq_' ->
+  subrelation (going eq_) (going eq_').
+Proof. intros ? ? ? []; eauto. Qed.
+
+#[global] Instance Equivalence_going :
+  Equivalence eq_ -> Equivalence (going eq_).
+Proof.
+  intros []; constructor; cbv; eauto.
+  - intros ? ? []; auto.
+  - intros ? ? ? [] []; eauto.
+Qed.
+
+End going_relations.
+
+Local Open Scope ctree_scope.
+
+(* Resum lemmas *)
+Lemma resumCtree_Ret {E1 E2 : Type} `{ReSumRet E1 E2}
+           {R} (r : R) :
+  resumCtree (Ret r) ≅ Ret r.
+Proof. step. cbn. constructor. reflexivity. Qed.
+
+Lemma resumCtree_Br  {E1 E2 : Type} `{ReSumRet E1 E2}
+           {R} (t : ctree E1 R) (n: nat) (k: fin' n -> ctree E1 R):
+  resumCtree (Br n k) ≅ Br n (fun x => resumCtree (k x)).
+Proof.
+  step.
+  cbn.
+  constructor.
+  intros.
+  reflexivity.
+Qed.
+
+Lemma resumCtree_Vis {E1 E2 : Type} `{ReSumRet E1 E2}
+           {R} (e : E1) (k : encode e -> ctree E1 R) :
+  resumCtree (Vis e k) ≅ Vis (resum e) (fun x => resumCtree (k (resum_ret e x))).
+Proof.
+  step.
+  cbn.
+  constructor.
+  intros.
+  reflexivity.
+Qed.
+
+(*| Dependent inversion of [equ] and [equb] equations |*)
+Lemma equ_ret_inv {E R} {HE: Encode E} {r1 r2 : R} :
+  (Ret r1) ≅ (Ret r2 : ctree E R) ->
+  r1 = r2.
+Proof.
+  intros EQ. step in EQ.
+  inv EQ; auto.
+Qed.
+
+Lemma equ_vis_invT {E S} {HE: Encode E} {e1 e2: E} {k1: encode e1 -> ctree E S} {k2: encode e2 -> ctree E S}:
+  Vis e1 k1 ≅ Vis e2 k2 ->
+  encode e1 = encode e2 /\ e1 = e2.
+Proof.
+  intros EQ. step in EQ.
+  inv EQ; auto.
+Qed.
+
+Lemma equ_vis_invE {E S} {HE: Encode E} {e: E} {k1 k2: encode e -> ctree E S}:
+  Vis e k1 ≅ Vis e k2 ->
+  forall x, k1 x ≅ k2 x.
+Proof.
+  intros EQ. step in EQ.
+  inv EQ.
+  dependent destruction H2.
+  auto.
+Qed.
+
+Lemma equ_br_invT {E S n1 n2} {HE: Encode E}
+  {k1 : fin' n1 -> ctree E S} {k2: fin' n2 -> ctree E S}:
+  Br n1 k1 ≅ Br n2 k2 ->
+  n1 = n2.
+Proof.
+  intros EQ; step in EQ.
+  inv EQ; auto.
+Qed.
+
+Lemma equ_br_invE {E S n} {HE: Encode E} {k1 k2: fin' n -> ctree E S}:
+  Br n k1 ≅ Br n k2 ->
+  forall x,k1 x ≅ k2 x.
+Proof.
+  intros EQ; step in EQ; cbn in EQ.
+  dependent destruction EQ.
+  auto.
+Qed.
+
+Lemma equ_tau_invE {E S} {HE: Encode E} {t1 t2: ctree E S}:
+  Tau t1 ≅ Tau t2 ->
+  t1 ≅ t2.
+Proof.
+  intros EQ; step in EQ; cbn in EQ.
+  now dependent destruction EQ.
+Qed.
+
+Lemma equF_vis_invT {E S} {HE: Encode E} {e1 e2: E} {R} {k1 k2: _ -> ctree E S}:
+  equF R (equ R) (VisF e1 k1) (VisF e2 k2) ->
+  encode e1 = encode e2 /\ e1 = e2.
+Proof.
+  intros EQ.
+  dependent induction EQ; auto.
+Qed.
+
+Lemma equF_vis_invE {E S} {HE: Encode E} {e: E} {R} {k1 k2 : _ -> ctree E S}:
+  equF R (equ R) (VisF e k1) (VisF e k2) ->
+  forall x, equ R (k1 x) (k2 x).
+Proof.
+  intros EQ.
+  inv EQ.
+  dependent destruction H1; dependent destruction H2; eauto.
+Qed.
+
+Lemma equF_br_invT {E S n1 n2} {HE: Encode E} {R}
+  (k1 : fin' n1 -> ctree E S) (k2: fin' n2 -> ctree E S) :
+  equF R (equ R) (BrF n1 k1) (BrF n2 k2) ->
+  n1 = n2.
+Proof.
+  intros EQ; dependent induction EQ; auto.
+Qed.
+
+Lemma equb_br_invE {E S n} {HE: Encode E} {R} {k1 k2: fin' n -> ctree E S}:
+  equF R (equ R) (BrF n k1) (BrF n k2) ->
+  forall x, equ R (k1 x) (k2 x).
+Proof.
+  intros EQ.
+  now dependent destruction EQ.
+Qed.
+
+(*|
+Proper Instances
+----------------
+TODO: step back and think a bit better about those
+
+equ eq       ==> going (equ eq)  observe
+∀(equ eq)    ==> going (equ eq)  BrF
+∀(equ eq)    ==> going (equ eq)  VisF
+observing eq --> equ eq
+going(equ)   ==> eq ==> fimpl    equb eq (t_equ eq r)
+eq ==> going(equ)   ==> fimpl    equb eq (t_equ eq r)
+equ ==> equ ==> flip impl)       bt_equ eq r
+|*)
+
+#[global] Instance equ_observe {E X} {HE: Encode E} {R: rel X X}: (* Why not X Y *)
+  Proper (equ R ==> going (equ R)) observe.
+Proof. constructor; step in H; now step. Qed.
+
+#[global] Instance equ_BrF {E X} {HE: Encode E} {n R}:
+  Proper (pointwise_relation _ (equ R) ==> going (equ R)) (@BrF E _ X _ n).
+Proof. constructor; red in H; step; econstructor; eauto. Qed.
+
+#[global] Instance equ_VisF {E X} {HE: Encode E} {R} (e : E) :
+  Proper (pointwise_relation _ (equ R) ==> going (equ R)) (@VisF E _ X _ e).
+Proof. constructor; step; constructor; eauto. Qed.
+
+(*| TODO: Here only [eq] is polymorphic enough to take both [ctree' E X] and [X] arguments |*)
+#[global] Instance observing_sub_equ_eq {E X} {HE: Encode E}:
+  subrelation (@observing E X _ eq) (equ eq).
+Proof.
+  repeat intro.
+  step; cbn; rewrite (observing_observe H); eauto.
+Qed.
+
+#[global] Instance equ_eq_equt {E X} {HE: Encode E} {r R} {HR: Equivalence R}:
+  Proper (going (equ R) ==> eq ==> flip impl)
+	     (@equF E _ X X R (et R r)).
+Proof.
+  unfold Proper, respectful, flip, impl; intros; subst.
+  inv H; step in H0; inv H0; inv H1; cbn in *; subst;
+  match goal with
+    | [H: ?a = ?b |- _] =>
+        match type of a with
+        | ctree' ?E ?X => inv H
+        end
+  end.
+  - econstructor; transitivity x1; eauto.
+  - dependent induction H4; econstructor.
+    now setoid_rewrite <- H in H0.
+  - econstructor.
+    transitivity t0; eauto.
+    now setoid_rewrite <- H.
+  - dependent induction H4; econstructor.
+    now setoid_rewrite <- H in H0.
+Qed.
+
+#[global] Instance equ_clos_eT_goal {E X} {HE: Encode E} R RR f {HR: Equivalence R}:
+  Proper (@equ E HE X X R ==> equ R ==> iff) (eT R f RR).
+Proof.
+  split; intros.
+  - rewrite <- H, <- H0; auto.
+  - rewrite H, H0; auto.
+Qed.
+
+#[global] Instance gfp_bt_equ {E X} {HE: Encode E} {r R} {HR: Equivalence R}:
+  Proper (@equ E HE X X R ==> equ R ==> iff) (ebt R r).
+Proof.
+  unfold Proper, respectful, flip, impl.
+  split; intros.
+  - etransitivity; [|etransitivity]; [|apply H1 |]; step.
+    + symmetry; assumption.
+    + assumption.
+  - etransitivity; [|etransitivity]; [|apply H1 |]; step.
+    + assumption.
+    + symmetry; assumption.
+Qed.
+
+#[global] Instance Equivalence_bt_equb_gen {E X} {HE: Encode E} {r R} {HR: Equivalence R}:
+  Proper ((gfp (@fequ E HE X X R)) ==> (gfp (@fequ E HE X X R)) ==> flip impl) (ebt R r).
+Proof.
+  unfold Proper, respectful, flip, impl.
+  intros.
+  etransitivity; [|etransitivity]; [| eassumption |];
+    step; [rewrite H|rewrite H0]; reflexivity.
+Qed.
